theories/data_lang/rsim/rules.v
@@ -156,7 +156,7 @@ Section sim_GS.
       - iDestruct "Hrsim12" as "(_ & Hrsim2)". iSmash.
     Qed.
 
-    Lemma rsim_constr Φ tag eₛ1 eₛ2 eₜ1 eₜ2 :
+    Lemma rsim_block Φ tag eₛ1 eₛ2 eₜ1 eₜ2 :
       SIM eₛ1 ⩾ eₜ1 [[ Χ ]] {{ sim_post_vals' (≈) }} -∗
       SIM eₛ2 ⩾ eₜ2 [[ Χ ]] {{ sim_post_vals' (≈) }} -∗
       ( ∀ vₛ vₜ,
@@ -166,9 +166,9 @@ Section sim_GS.
       SIM &tag eₛ1 eₛ2 ⩾ &tag eₜ1 eₜ2 [[ Χ ]] {{ Φ }}.
     Proof.
       iIntros "Hrsim1 Hrsim2 HΦ". rsim_intro.
-      sim_apply (sim_constr with "(Hrsim1 [//] HΓ) (Hrsim2 [//] HΓ)").
+      sim_apply (sim_block with "(Hrsim1 [//] HΓ) (Hrsim2 [//] HΓ)").
     Qed.
-    Lemma rsim_constr_valₜ1 Φ tag eₛ vₜ1 eₜ :
+    Lemma rsim_block_valₜ1 Φ tag eₛ vₜ1 eₜ :
       SIM eₛ ⩾ eₜ [[ Χ ]] {{ sim_post_vals' (≈) }} -∗
       ( ∀ vₛ lₜ vₜ,
         (lₜ +ₗ 0) ↦ₜ tag -∗
@@ -180,9 +180,9 @@ Section sim_GS.
       SIM eₛ ⩾ &tag vₜ1 eₜ [[ Χ ]] {{ Φ }}.
     Proof.
       iIntros "Hrsim HΦ". rsim_intro.
-      sim_apply (sim_constr_valₜ1 with "(Hrsim [//] HΓ)").
+      sim_apply (sim_block_valₜ1 with "(Hrsim [//] HΓ)").
     Qed.
-    Lemma rsim_constr_valₜ2 Φ tag eₛ eₜ vₜ2 :
+    Lemma rsim_block_valₜ2 Φ tag eₛ eₜ vₜ2 :
       SIM eₛ ⩾ eₜ [[ Χ ]] {{ sim_post_vals' (≈) }} -∗
       ( ∀ vₛ lₜ vₜ,
         (lₜ +ₗ 0) ↦ₜ tag -∗
@@ -194,7 +194,7 @@ Section sim_GS.
       SIM eₛ ⩾ &tag eₜ vₜ2 [[ Χ ]] {{ Φ }}.
     Proof.
       iIntros "Hrsim HΦ". rsim_intro.
-      sim_apply (sim_constr_valₜ2 with "(Hrsim [//] HΓ)").
+      sim_apply (sim_block_valₜ2 with "(Hrsim [//] HΓ)").
     Qed.
 
     Lemma rsim_load Φ eₛ1 eₛ2 eₜ1 eₜ2 :
@@ -345,7 +345,7 @@ Section sim_GS.
       iApply (rsim_if with "Hrsim0 Hrsim12").
     Qed.
 
-    Lemma rsimv_constr Φ tag eₛ1 eₛ2 eₜ1 eₜ2 :
+    Lemma rsimv_block Φ tag eₛ1 eₛ2 eₜ1 eₜ2 :
       SIM eₛ1 ⩾ eₜ1 [[ Χ ]] {{# (≈) }} -∗
       SIM eₛ2 ⩾ eₜ2 [[ Χ ]] {{# (≈) }} -∗
       ( ∀ vₛ vₜ,
@@ -356,10 +356,10 @@ Section sim_GS.
     Proof.
       rewrite !rsimv_unseal.
       iIntros "Hrsim1 Hrsim2 HΦ".
-      iApply (rsim_constr with "Hrsim1 Hrsim2").
+      iApply (rsim_block with "Hrsim1 Hrsim2").
       rewrite /sim_post_vals'. iSmash.
     Qed.
-    Lemma rsimv_constr_valₜ1 Φ tag eₛ vₜ1 eₜ :
+    Lemma rsimv_block_valₜ1 Φ tag eₛ vₜ1 eₜ :
       SIM eₛ ⩾ eₜ [[ Χ ]] {{# (≈) }} -∗
       ( ∀ vₛ lₜ vₜ,
         (lₜ +ₗ 0) ↦ₜ tag -∗
@@ -372,10 +372,10 @@ Section sim_GS.
     Proof.
       rewrite !rsimv_unseal.
       iIntros "Hrsim HΦ".
-      iApply (rsim_constr_valₜ1 with "Hrsim").
+      iApply (rsim_block_valₜ1 with "Hrsim").
       rewrite /sim_post_vals'. iSmash.
     Qed.
-    Lemma rsimv_constr_valₜ2 Φ tag eₛ eₜ vₜ2 :
+    Lemma rsimv_block_valₜ2 Φ tag eₛ eₜ vₜ2 :
       SIM eₛ ⩾ eₜ [[ Χ ]] {{# (≈) }} -∗
       ( ∀ vₛ lₜ vₜ,
         (lₜ +ₗ 0) ↦ₜ tag -∗
@@ -388,7 +388,7 @@ Section sim_GS.
     Proof.
       rewrite !rsimv_unseal.
       iIntros "Hrsim HΦ".
-      iApply (rsim_constr_valₜ2 with "Hrsim").
+      iApply (rsim_block_valₜ2 with "Hrsim").
       rewrite /sim_post_vals'. iSmash.
     Qed.
 
